Remove useless uniquization
We instead typeclass-resolve a proof that the given list is already
unique.  This will hopefully make the JSON parser reduce more quickly.

src/Parsers/ParserFromParserADT.v
@@ -27,7 +27,8 @@ Section parser.
   Context {stringlike_stringlikemin : StringLikeMin Ascii.ascii}
           {stringlike_stringlike : StringLike Ascii.ascii}
           {stringlike_stringlike_properties : StringLikeProperties Ascii.ascii}.
-  Context {ls : list (String.string * productions Ascii.ascii)}.
+  Context {ls : list (String.string * productions Ascii.ascii)}
+          {HNoDup : NoDupR Equality.string_beq (List.map fst ls)}.
   Local Notation G := (list_to_grammar nil ls) (only parsing).
   Context (Hvalid : is_true (grammar_rvalid G)).
   Context (splitter_impl : FullySharpened (string_spec G stringlike_stringlike)).
@@ -79,7 +80,7 @@ Section parser.
 
   Definition parser' : Parser G stringlike_stringlike.
   Proof.
-    refine (@parser ls Hvalid (adt_based_splitter splitter_impl)
+    refine (@parser ls HNoDup Hvalid (adt_based_splitter splitter_impl)
                     (adt_based_StringLikeMin_lite splitter_impl)
                     _
                     _
@@ -109,10 +110,10 @@ End parser.
 
 Definition parser''
            {HSLM HSL HSLP}
-           {ls}
+           {ls HNoDup}
            Hvalid
            splitter_impl
-           val (H : val = has_parse (@parser' HSLM HSL HSLP ls Hvalid splitter_impl))
+           val (H : val = has_parse (@parser' HSLM HSL HSLP ls HNoDup Hvalid splitter_impl))
 : Parser (list_to_grammar nil ls) HSL.
 Proof.
   refine {| has_parse := val |};
@@ -184,17 +185,44 @@ Definition parser
            {HSL : StringLike Ascii.ascii}
            {HSLP : StringLikeProperties Ascii.ascii}
            {ls : list (string * productions Ascii.ascii)}
+           {HNoDup : NoDupR Equality.string_beq (List.map fst ls)}
            (Hvalid : is_true (grammar_rvalid (list_to_grammar nil ls)))
            (splitter_impl : FullySharpened (string_spec (list_to_grammar nil ls) HSL))
 : Parser (list_to_grammar nil ls) HSL.
 Proof.
-  let term := (eval cbv beta delta [parser''] in (@parser'' HSLM HSL HSLP ls Hvalid splitter_impl)) in
+  let term := (eval cbv beta delta [parser''] in (@parser'' HSLM HSL HSLP ls HNoDup Hvalid splitter_impl)) in
   refine (term _ _).
   cbv beta iota zeta delta [has_parse parser' parser transfer_parser new_string_of_string proj adtProj proj1_sig new_string_of_base_string cConstructors StringLike.length adt_based_StringLikeMin adt_based_StringLikeMin_lite adt_based_StringLike_lite pdata BaseTypes.split_string_for_production split_dataProj adt_based_splitter BuildComputationalADT.callcADTMethod ibound indexb cMethods cRep BaseTypes.predata ParserImplementation.parser_data adt_based_StringLike RDPList.rdp_list_predata RDPList.rdp_list_nonterminals_listT list_to_grammar Valid_nonterminals RDPList.rdp_list_is_valid_nonterminal RDPList.rdp_list_remove_nonterminal list_to_productions newS Fin.R mto_string msplits drop take is_char String length get bool_eq beq mlength mchar_at_matches mdrop mtake mget].
   change_opt ls nt str.
-  match goal with
-    | [ |- _ = ?x :> ?T ] => instantiate (1 := x); exact_no_check (@eq_refl T x)
+  lazymatch goal with
+    | [ |- appcontext[BooleanRecognizerOptimized.opt.opt.id
+                        (BooleanRecognizerOptimized.opt.opt.first_index_default
+                           ?a ?b
+                           (BooleanRecognizerOptimized.opt.opt.map
+                              BooleanRecognizerOptimized.opt.opt.fst ls))] ]
+      => replace (BooleanRecognizerOptimized.opt.opt.id
+                    (BooleanRecognizerOptimized.opt.opt.first_index_default
+                       a
+                       b
+                       (BooleanRecognizerOptimized.opt.opt.map
+                          BooleanRecognizerOptimized.opt.opt.fst ls)))
+         with (BooleanRecognizerOptimized.opt.opt.list_caset
+                 (fun _ => _)
+                 b
+                 (fun _ _ => 0)
+                 ls)
   end.
+  { match goal with
+      | [ |- _ = ?x :> ?T ] => instantiate (1 := x); exact_no_check (@eq_refl T x)
+    end. }
+  { abstract (
+        clear;
+        destruct ls; unfold BooleanRecognizerOptimized.opt.opt.first_index_default, BooleanRecognizerOptimized.opt.opt.id; simpl;
+        [ reflexivity | ];
+        change @BooleanRecognizerOptimized.opt.opt.string_beq with Equality.string_beq;
+        rewrite Equality.string_lb by reflexivity;
+        reflexivity
+      ). }
 Defined.
 
-Global Arguments parser {HSLM HSL HSLP} {ls} Hvalid splitter_impl / .
+Global Arguments parser {HSLM HSL HSLP} {ls HNoDup} Hvalid splitter_impl / .
